theories/Tactics.v
@@ -23,15 +23,15 @@ Ltac reshape_expr_ordered b e tac :=
       | false => tac K e
       | true  => fail
       end
-  | App ?e1 ?e2 => reshape_val e1 ltac:(fun v1 => go (AppRCtx v1 :: K) e2)
-  | App ?e1 ?e2 => go (AppLCtx e2 :: K) e1
+  | App ?e1 ?e2 => reshape_val e2 ltac:(fun v2 => go (AppLCtx v2 :: K) e1)
+  | App ?e1 ?e2 => go (AppRCtx e1 :: K) e2
   | UnOp ?op ?e => go (UnOpCtx op :: K) e
   | BinOp ?op ?e1 ?e2 =>
-     reshape_val e1 ltac:(fun v1 => go (BinOpRCtx op v1 :: K) e2)
-  | BinOp ?op ?e1 ?e2 => go (BinOpLCtx op e2 :: K) e1
+     reshape_val e2 ltac:(fun v2 => go (BinOpLCtx op v2 :: K) e1)
+  | BinOp ?op ?e1 ?e2 => go (BinOpRCtx op e1 :: K) e2
   | If ?e0 ?e1 ?e2 => go (IfCtx e1 e2 :: K) e0
-  | Pair ?e1 ?e2 => reshape_val e1 ltac:(fun v1 => go (PairRCtx v1 :: K) e2)
-  | Pair ?e1 ?e2 => go (PairLCtx e2 :: K) e1
+  | Pair ?e1 ?e2 => reshape_val e2 ltac:(fun v2 => go (PairLCtx v2 :: K) e1)
+  | Pair ?e1 ?e2 => go (PairRCtx e1 :: K) e2
   | Fst ?e => go (FstCtx :: K) e
   | Snd ?e => go (SndCtx :: K) e
   | InjL ?e => go (InjLCtx :: K) e
@@ -39,14 +39,14 @@ Ltac reshape_expr_ordered b e tac :=
   | Case ?e0 ?e1 ?e2 => go (CaseCtx e1 e2 :: K) e0
   | Alloc ?e => go (AllocCtx :: K) e
   | Load ?e => go (LoadCtx :: K) e
-  | Store ?e1 ?e2 => reshape_val e1 ltac:(fun v1 => go (StoreRCtx v1 :: K) e2)
-  | Store ?e1 ?e2 => go (StoreLCtx e2 :: K) e1
-  | CAS ?e0 ?e1 ?e2 => reshape_val e0 ltac:(fun v0 => first
-     [ reshape_val e1 ltac:(fun v1 => go (CasRCtx v0 v1 :: K) e2)
-     | go (CasMCtx v0 e2 :: K) e1 ])
-  | CAS ?e0 ?e1 ?e2 => go (CasLCtx e1 e2 :: K) e0
-  | FAA ?e1 ?e2 => reshape_val e1 ltac:(fun v1 => go (FaaRCtx v1 :: K) e2)
-  | FAA ?e1 ?e2 => go (FaaLCtx e2 :: K) e1
+  | Store ?e1 ?e2 => reshape_val e2 ltac:(fun v2 => go (StoreLCtx v2 :: K) e1)
+  | Store ?e1 ?e2 => go (StoreRCtx e1 :: K) e2
+  | CAS ?e0 ?e1 ?e2 => reshape_val e2 ltac:(fun v2 => first
+     [ reshape_val e1 ltac:(fun v1 => go (CasLCtx v1 v2 :: K) e0)
+     | go (CasMCtx e0 v2 :: K) e1 ])
+  | CAS ?e0 ?e1 ?e2 => go (CasRCtx e0 e1 :: K) e2
+  | FAA ?e1 ?e2 => reshape_val e2 ltac:(fun v2 => go (FaaLCtx v2 :: K) e1)
+  | FAA ?e1 ?e2 => go (FaaRCtx e1 :: K) e2
   | _ =>
       lazymatch b with
       | false => fail
@@ -59,7 +59,7 @@ Local Lemma head_step_into_val e σ e' v' σ' efs :
   head_step e σ (of_val v') σ' efs →
   head_step e σ e' σ' efs.
 Proof.
-  intros Hval Hstep. by erewrite of_to_val in Hstep.
+  intros Hval Hstep. by rewrite Hval in Hstep.
 Qed.
 
 Ltac prim_step :=
@@ -67,7 +67,7 @@ Ltac prim_step :=
   | |- prim_step ?e _ _ _ _ =>
       reshape_expr_ordered true e ltac:(fun K e' =>
         esplit with K e' _ ; [ reflexivity | reflexivity | ] ;
-        (idtac + eapply head_step_into_val) ; econstructor
+        (idtac + (eapply head_step_into_val; [apply _|])) ; econstructor
       )
   end ;
   simpl_to_of_val.
